disk-betree/ImplState.i.dfy
@@ -2,6 +2,7 @@ include "../lib/MutableMap.i.dfy"
 include "ImplModel.i.dfy"
 include "MainDiskIOHandler.s.dfy"
 include "MutableBucket.i.dfy"
+include "ImplNodes.i.dfy"
 
 module {:extern} ImplState {
   import opened Options
@@ -9,6 +10,8 @@ module {:extern} ImplState {
   import opened NativeTypes
   import TTT = TwoThreeTree
   import IM = ImplModel
+  import opened ImplNode
+  import opened ImplMutCache
 
   import BT = PivotBetreeSpec`Internal
   import Messages = ValueMessage
@@ -32,71 +35,8 @@ module {:extern} ImplState {
   type Message = Messages.Message
   type TreeMap = TTT.Tree<Message>
 
-  type MutIndirectionTable = MM.ResizingHashMap<(Option<BC.Location>, seq<Reference>)>
+  type MutIndirectionTable = MM.ResizingHashMap<(Option<BC.Location>, seq<BT.G.Reference>)>
   type MutIndirectionTableNullable = MM.ResizingHashMap?<(Option<BC.Location>, seq<Reference>)>
-
-  datatype Node = Node(
-      pivotTable: Pivots.PivotTable,
-      children: Option<seq<Reference>>,
-      buckets: seq<MutableBucket.MutBucket>
-    )
-
-  type MutCache = MM.ResizingHashMap<Node>
-
-  function BucketListObjectSet(s: seq<MutableBucket.MutBucket>) : set<object>
-  {
-    set i | 0 <= i < |s| :: s[i]
-  }
-
-  function BucketListRepr(s: seq<MutableBucket.MutBucket>) : set<object>
-  reads BucketListObjectSet(s)
-  {
-    set i, o | 0 <= i < |s| && o in s[i].Repr :: o
-  }
-
-  predicate {:opaque} BucketListReprInv(buckets: seq<MutableBucket.MutBucket>)
-  reads BucketListObjectSet(buckets)
-  {
-    forall i, j | 0 <= i < |buckets| && 0 <= j < |buckets| && i != j ::
-        buckets[i].Repr !! buckets[j].Repr
-  }
-
-  function NodeObjectSet(node: Node) : set<object>
-  {
-    set i | 0 <= i < |node.buckets| :: node.buckets[i]
-  }
-
-  function NodeRepr(node: Node) : set<object>
-  reads NodeObjectSet(node)
-  {
-    set i, o | 0 <= i < |node.buckets| && o in node.buckets[i].Repr :: o
-  }
-
-  function CacheObjectSet(cache: map<BT.G.Reference, Node>) : set<object>
-  {
-    set ref, i | ref in cache && 0 <= i < |cache[ref].buckets| :: cache[ref].buckets[i]
-  }
-
-  function {:opaque} CacheRepr(cache: map<BT.G.Reference, Node>) : set<object>
-  reads CacheObjectSet(cache)
-  {
-    set ref, i, o | ref in cache && 0 <= i < |cache[ref].buckets| && o in cache[ref].buckets[i].Repr :: o
-  }
-
-  predicate WFNode(node: Node)
-  reads set i | 0 <= i < |node.buckets| :: node.buckets[i]
-  reads set i, o | 0 <= i < |node.buckets| && o in node.buckets[i].Repr :: o
-  {
-    forall i | 0 <= i < |node.buckets| :: node.buckets[i].Inv()
-  }
-
-  function INode(node: Node) : IM.Node
-  reads set i | 0 <= i < |node.buckets| :: node.buckets[i]
-  reads set i, o | 0 <= i < |node.buckets| && o in node.buckets[i].Repr :: o
-  {
-    IM.Node(node.pivotTable, node.children,
-      MutableBucket.MutBucket.ISeq(node.buckets))
-  }
 
   datatype Sector =
     | SectorBlock(block: Node)
@@ -104,15 +44,18 @@ module {:extern} ImplState {
 
   function SectorObjectSet(sector: Sector) : set<object>
   {
-    if sector.SectorIndirectionTable? then {sector.indirectionTable} else NodeObjectSet(sector.block)
+    match sector {
+      case SectorIndirectionTable(indirectionTable) => {indirectionTable}
+      case SectorBlock(block) => {block}
+    }
   }
 
   function SectorRepr(sector: Sector) : set<object>
-  reads SectorObjectSet(sector)
+  reads if sector.SectorIndirectionTable? then {sector.indirectionTable} else {sector.block}
   {
     match sector {
       case SectorIndirectionTable(indirectionTable) => {indirectionTable} + indirectionTable.Repr
-      case SectorBlock(block) => NodeRepr(block)
+      case SectorBlock(block) => block.Repr
     }
   }
  
@@ -121,10 +64,7 @@ module {:extern} ImplState {
   reads SectorRepr(sector)
   {
     && (sector.SectorIndirectionTable? ==> sector.indirectionTable.Inv())
-    && (sector.SectorBlock? ==>
-      && WFNode(sector.block)
-      && BucketListReprInv(sector.block.buckets)
-    )
+    && (sector.SectorBlock? ==> sector.block.Inv())
   }
 
   function IIndirectionTable(table: MutIndirectionTable) : (result: IM.IndirectionTable)
@@ -132,14 +72,6 @@ module {:extern} ImplState {
   {
     table.Contents
   }
- 
-  /*function ICache(table: MutCache) : (result: map<BT.G.Reference, IM.Node>)
-  reads table, table.Repr
-  reads set ref, i | ref in table.Contents && 0 <= i < |table.Contents[ref].buckets| :: table.Contents[ref].buckets[i]
-  reads set ref, i, o | ref in table.Contents && 0 <= i < |table.Contents[ref].buckets| && o in table.Contents[ref].buckets[i].Repr :: o
-  {
-      map ref | ref in table.Contents :: INode(table.Contents[ref])
-  }*/
  
   function IIndirectionTableOpt(table: MutIndirectionTableNullable) : (result: Option<IM.IndirectionTable>)
   reads if table != null then {table} + table.Repr else {}
@@ -152,60 +84,16 @@ module {:extern} ImplState {
  
   function ISector(sector: Sector) : IM.Sector
   requires WFSector(sector)
-  reads if sector.SectorIndirectionTable? then sector.indirectionTable.Repr else {}
-  reads if sector.SectorBlock?
-      then set i | 0 <= i < |sector.block.buckets| :: sector.block.buckets[i]
-      else {}
-  reads if sector.SectorBlock?
-      then set i, o | 0 <= i < |sector.block.buckets| && o in sector.block.buckets[i].Repr :: o
-      else {}
+  reads if sector.SectorIndirectionTable? then {sector.indirectionTable} else {sector.block}
+  reads SectorRepr(sector)
   {
     match sector {
-      case SectorBlock(node) => IM.SectorBlock(INode(node))
+      case SectorBlock(node) => IM.SectorBlock(node.I())
       case SectorIndirectionTable(indirectionTable) => IM.SectorIndirectionTable(IIndirectionTable(indirectionTable))
     }
   }
 
-  // These functions are all pulled out so that we can avoid having `reads this` on them.
-
-  predicate {:opaque} BucketsInv_(contents: map<BT.G.Reference, Node>, BucketObjects: set<object>, BucketRepr: set<object>)
-  reads BucketObjects, BucketRepr
-  requires BucketObjects == CacheObjectSet(contents)
-  requires BucketRepr == CacheRepr(contents)
-  {
-    reveal_CacheRepr();
-    (forall ref, i | ref in contents && 0 <= i < |contents[ref].buckets| ::
-      && contents[ref].buckets[i].Inv())
-  }
-
-  function {:opaque} Cache_(cache: MutCache, BucketObjects: set<object>, BucketRepr: set<object>) : map<BT.G.Reference, IM.Node>
-  reads cache, BucketObjects, BucketRepr
-  requires BucketObjects == CacheObjectSet(cache.Contents)
-  requires BucketRepr == CacheRepr(cache.Contents)
-  ensures forall ref | ref in cache.Contents :: ref in Cache_(cache, BucketObjects, BucketRepr)
-  ensures forall ref | ref in cache.Contents :: 
-      Cache_(cache, BucketObjects, BucketRepr)[ref] == INode(cache.Contents[ref])
-  {
-    reveal_CacheRepr();
-    map ref | ref in cache.Contents :: INode(cache.Contents[ref])
-  }
-
-  predicate {:opaque} CacheReprInv_(contents: map<BT.G.Reference, Node>, BucketObjects: set<object>) 
-  reads BucketObjects
-  requires BucketObjects == CacheObjectSet(contents)
-  {
-    && (forall ref1, i1, ref2, i2 | ref1 in contents && ref2 in contents
-        && 0 <= i1 < |contents[ref1].buckets|
-        && 0 <= i2 < |contents[ref2].buckets|
-        && (ref1 != ref2 || i1 != i2) ::
-        contents[ref1].buckets[i1].Repr !! contents[ref2].buckets[i2].Repr)
-  }
-
-
   class Variables {
-    ghost var BucketObjects: set<object>;
-    ghost var BucketRepr: set<object>;
-
     var ready: bool;
 
     var syncReqs: map<int, BC.SyncReqStatus>;
@@ -223,14 +111,7 @@ module {:extern} ImplState {
     // Unready
     var outstandingIndirectionTableRead: Option<D.ReqId>;
 
-    predicate CacheReprInv() 
-    reads this, cache, BucketObjects
-    requires BucketObjects == CacheObjectSet(cache.Contents)
-    {
-      CacheReprInv_(cache.Contents, BucketObjects)
-    }
-
-    function NonBucketsRepr() : set<object>
+    function Repr() : set<object>
     reads this, persistentIndirectionTable, ephemeralIndirectionTable,
         frozenIndirectionTable, lru, cache
     {
@@ -242,28 +123,12 @@ module {:extern} ImplState {
       cache.Repr
     }
 
-    function Repr() : set<object>
-    reads this, persistentIndirectionTable, ephemeralIndirectionTable,
-        frozenIndirectionTable, lru, cache, BucketObjects
-    {
-      {this} +
-      persistentIndirectionTable.Repr +
-      ephemeralIndirectionTable.Repr +
-      (if frozenIndirectionTable != null then frozenIndirectionTable.Repr else {}) +
-      lru.Repr +
-      cache.Repr +
-      BucketRepr
-    }
-
     predicate ReprInv()
     reads this, persistentIndirectionTable, ephemeralIndirectionTable,
-        frozenIndirectionTable, lru, cache, BucketObjects
+        frozenIndirectionTable, lru, cache
     reads Repr()
     {
         // NOALIAS statically enforced no-aliasing would probably help here
-        && BucketObjects == CacheObjectSet(cache.Contents)
-        && BucketRepr == CacheRepr(cache.Contents)
-        && BucketObjects <= BucketRepr
 
         && persistentIndirectionTable.Repr !! ephemeralIndirectionTable.Repr
         && (frozenIndirectionTable != null ==> persistentIndirectionTable.Repr !! frozenIndirectionTable.Repr)
@@ -276,33 +141,16 @@ module {:extern} ImplState {
         && (frozenIndirectionTable != null ==> cache.Repr !! frozenIndirectionTable.Repr)
         && cache.Repr !! lru.Repr
 
-        && persistentIndirectionTable.Repr !! BucketRepr
-        && (frozenIndirectionTable != null ==> frozenIndirectionTable.Repr !! BucketRepr)
-        && ephemeralIndirectionTable.Repr !! BucketRepr
-        && cache.Repr !! BucketRepr
-        && lru.Repr !! BucketRepr
-        && CacheReprInv()
-
         && this !in ephemeralIndirectionTable.Repr
         && this !in persistentIndirectionTable.Repr
         && (frozenIndirectionTable != null ==> this !in frozenIndirectionTable.Repr)
         && this !in lru.Repr
         && this !in cache.Repr
-        && this !in BucketRepr
-    }
-
-    predicate BucketsInv()
-    reads this, cache
-    reads BucketObjects, BucketRepr
-    requires BucketObjects == CacheObjectSet(cache.Contents)
-    requires BucketRepr == CacheRepr(cache.Contents)
-    {
-      BucketsInv_(cache.Contents, BucketObjects, BucketRepr)
     }
 
     predicate W()
     reads this, persistentIndirectionTable, ephemeralIndirectionTable,
-        frozenIndirectionTable, lru, cache, BucketObjects
+        frozenIndirectionTable, lru, cache
     reads Repr()
     {
       && ReprInv()
@@ -311,26 +159,16 @@ module {:extern} ImplState {
       && ephemeralIndirectionTable.Inv()
       && lru.Inv()
       && cache.Inv()
-      && BucketsInv()
-    }
-
-    function Cache() : map<BT.G.Reference, IM.Node>
-    reads this, cache
-    reads BucketObjects, BucketRepr
-    requires BucketObjects == CacheObjectSet(cache.Contents)
-    requires BucketRepr == CacheRepr(cache.Contents)
-    {
-      Cache_(cache, BucketObjects, BucketRepr)
     }
 
     function I() : IM.Variables
     reads this, persistentIndirectionTable, ephemeralIndirectionTable,
-        frozenIndirectionTable, lru, cache, BucketObjects
+        frozenIndirectionTable, lru, cache
     reads Repr()
     requires W()
     {
       if ready then (
-        IM.Ready(IIndirectionTable(persistentIndirectionTable), IIndirectionTableOpt(frozenIndirectionTable), IIndirectionTable(ephemeralIndirectionTable), outstandingIndirectionTableWrite, outstandingBlockWrites, outstandingBlockReads, syncReqs, Cache(), lru.Queue)
+        IM.Ready(IIndirectionTable(persistentIndirectionTable), IIndirectionTableOpt(frozenIndirectionTable), IIndirectionTable(ephemeralIndirectionTable), outstandingIndirectionTableWrite, outstandingBlockWrites, outstandingBlockReads, syncReqs, cache.I(), lru.Queue)
       ) else (
         IM.Unready(outstandingIndirectionTableRead, syncReqs)
       )
@@ -338,7 +176,7 @@ module {:extern} ImplState {
 
     predicate WF()
     reads this, persistentIndirectionTable, ephemeralIndirectionTable,
-        frozenIndirectionTable, lru, cache, BucketObjects
+        frozenIndirectionTable, lru, cache
     reads Repr()
     {
       && W()
@@ -361,21 +199,13 @@ module {:extern} ImplState {
       ephemeralIndirectionTable := new MM.ResizingHashMap(128);
       persistentIndirectionTable := new MM.ResizingHashMap(128);
       frozenIndirectionTable := null;
-      cache := new MM.ResizingHashMap(128);
-
-      new;
-
-      BucketObjects := CacheObjectSet(cache.Contents);
-      BucketRepr := CacheRepr(cache.Contents);
-
-      reveal_CacheRepr();
-      reveal_CacheReprInv_();
+      cache := new MutCache();
     }
   }
 
   predicate Inv(k: M.Constants, s: Variables)
   reads s, s.persistentIndirectionTable, s.ephemeralIndirectionTable,
-        s.frozenIndirectionTable, s.lru, s.cache, s.BucketObjects
+        s.frozenIndirectionTable, s.lru, s.cache
   reads s.Repr()
   {
     && s.W()
@@ -401,53 +231,10 @@ module {:extern} ImplState {
 
   twostate predicate WellUpdated(s: Variables)
   reads s, s.persistentIndirectionTable, s.ephemeralIndirectionTable,
-      s.frozenIndirectionTable, s.lru, s.cache, s.BucketObjects
+      s.frozenIndirectionTable, s.lru, s.cache
   reads s.Repr()
   {
     && s.W()
     && (forall o | o in s.Repr() :: o in old(s.Repr()) || fresh(o))
-  }
-
-  // Some helpful lemmas
-
-  lemma LemmaCacheObjectSetLeRepr(cache: map<BT.G.Reference, Node>)
-  requires BucketsInv_(cache, CacheObjectSet(cache), CacheRepr(cache))
-  ensures CacheObjectSet(cache) <= CacheRepr(cache)
-  {
-    reveal_BucketsInv_();
-    reveal_Cache_();
-    reveal_CacheRepr();
-  }
-
-  lemma LemmaReprCacheInsert(cache: map<BT.G.Reference, Node>, ref: BT.G.Reference, node: Node, s: Variables)
-  requires s.cache.Contents == cache[ref := node]
-  requires CacheRepr(cache) !! NodeRepr(node)
-  requires CacheRepr(cache) !! s.NonBucketsRepr()
-  requires NodeRepr(node) !! s.NonBucketsRepr()
-  requires CacheReprInv_(cache, CacheObjectSet(cache))
-  requires BucketListReprInv(node.buckets)
-  ensures CacheRepr(s.cache.Contents) !! s.NonBucketsRepr()
-  ensures CacheReprInv_(s.cache.Contents, CacheObjectSet(s.cache.Contents))
-  ensures BucketsInv_(s.cache.Contents, CacheObjectSet(s.cache.Contents), CacheRepr(s.cache.Contents))
-
-  method CacheInsert(k: M.Constants, s: Variables, ref: BT.G.Reference, node: Node)
-  requires s.W()
-  requires s.ready
-  requires NodeRepr(node) !! s.Repr()
-  requires |s.cache.Contents| <= MaxCacheSize();
-  modifies s.Repr()
-  ensures s.W()
-  ensures forall o | o in s.Repr() :: fresh(o) || o in old(s.Repr()) || o in old(NodeRepr(node))
-  ensures s.I() == old(s.I()).(cache := old(s.I()).cache[ref := INode(node)])
-  {
-    var _ := s.cache.Insert(ref, node);
-
-    s.BucketObjects := CacheObjectSet(s.cache.Contents);
-    s.BucketRepr := CacheRepr(s.cache.Contents);
-
-    reveal_BucketListReprInv();
-    reveal_CacheRepr();
-    reveal_Cache_();
-    reveal_CacheReprInv_();
   }
 }
