disk-betree/ImplNodes.i.dfy
@@ -1,0 +1,220 @@
+include "../lib/MutableMap.i.dfy"
+include "ImplModel.i.dfy"
+include "MainDiskIOHandler.s.dfy"
+include "MutableBucket.i.dfy"
+
+module ImplNode {
+  import opened Options
+  import opened Sequences
+  import opened NativeTypes
+  import TTT = TwoThreeTree
+  import IM = ImplModel
+
+  import BT = PivotBetreeSpec`Internal
+  import Messages = ValueMessage
+  import MS = MapSpec
+  import Pivots = PivotsLib
+  import BC = BetreeGraphBlockCache
+  import D = AsyncSectorDisk
+  import MainDiskIOHandler
+  import LruModel
+  import MutableLru
+  import MutableBucket
+  import opened Bounds
+  import opened BucketsLib
+
+  import MM = MutableMap
+  import ReferenceType`Internal
+
+  predicate {:opaque} BucketListReprDisjoint(buckets: seq<MutableBucket.MutBucket>)
+  reads set i | 0 <= i < |buckets| :: buckets[i]
+  {
+    forall i, j | 0 <= i < |buckets| && 0 <= j < |buckets| && i != j ::
+        buckets[i].Repr !! buckets[j].Repr
+  }
+
+  class Node
+  {
+    var pivotTable: Pivots.PivotTable;
+    var children: Option<seq<BT.G.Reference>>;
+    var buckets: seq<MutableBucket.MutBucket>;
+    ghost var Repr: set<object>;
+
+    constructor(
+      pivotTable: Pivots.PivotTable,
+      children: Option<seq<BT.G.Reference>>,
+      buckets: seq<MutableBucket.MutBucket>)
+    requires forall i | 0 <= i < |buckets| :: buckets[i].Inv()
+    requires BucketListReprDisjoint(buckets)
+    ensures this.pivotTable == pivotTable;
+    ensures this.children == children;
+    ensures this.buckets == buckets;
+    ensures Inv();
+    {
+      this.pivotTable := pivotTable;
+      this.children := children;
+      this.buckets := buckets;
+
+      new;
+
+      this.Repr := {this} + ComputeRepr();
+    }
+
+    protected function ComputeRepr() : set<object>
+    reads this
+    reads set i | 0 <= i < |buckets| :: buckets[i]
+    {
+      set i, o | 0 <= i < |buckets| && o in buckets[i].Repr :: o
+    }
+
+
+    protected predicate Inv()
+    reads this, Repr
+    ensures Inv() ==> this in Repr
+    ensures Inv() ==>
+      forall i | 0 <= i < |buckets| :: buckets[i].Inv()
+    {
+      && (forall i | 0 <= i < |buckets| :: buckets[i] in Repr)
+      && Repr == {this} + ComputeRepr()
+      && BucketListReprDisjoint(buckets)
+
+      && (forall i | 0 <= i < |buckets| :: buckets[i].Inv())
+    }
+
+    function I() : IM.Node
+    reads this, Repr
+    requires Inv()
+    {
+      IM.Node(pivotTable, children,
+        MutableBucket.MutBucket.ISeq(buckets))
+    }
+  }
+}
+
+module ImplMutCache {
+  import opened ImplNode
+  import opened Options
+
+  // TODO ARARGHGHESGKSG it sucks that we have to wrap this in a new object type
+  // just to have a Repr field. It also sucks that we have to have a Repr field
+  // at all instead of an opaque Repr() function, see
+  // https://github.com/dafny-lang/dafny/issues/377
+  class MutCache
+  {
+    var cache: MM.ResizingHashMap<Node>;
+    ghost var Repr: set<object>;
+
+    constructor()
+    ensures Inv();
+    ensures I() == map[]
+    ensures fresh(Repr);
+    {
+      cache := new MM.ResizingHashMap(128);
+      new;
+      Repr := {this} + cache.Repr + MutCacheBucketRepr();
+    }
+
+    protected function MutCacheBucketRepr() : set<object>
+    reads this, cache
+    reads set ref | ref in cache.Contents :: cache.Contents[ref]
+    {
+      set ref, o | ref in cache.Contents && o in cache.Contents[ref].Repr :: o
+    }
+
+    protected predicate CacheReprDisjoint(contents: map<BT.G.Reference, Node>)
+    reads set ref | ref in contents :: contents[ref]
+    {
+      forall ref1, ref2 | ref1 in contents && ref2 in contents && 
+          ref1 != ref2 :: contents[ref1].Repr !! contents[ref2].Repr
+    }
+
+    protected predicate Inv()
+    reads this, Repr
+    ensures Inv() ==> this in Repr
+    {
+      && cache in Repr
+      && (forall ref | ref in cache.Contents :: cache.Contents[ref] in Repr)
+      && Repr == {this} + cache.Repr + MutCacheBucketRepr()
+      && CacheReprDisjoint(cache.Contents)
+      && (forall ref | ref in cache.Contents :: cache.Contents[ref].Repr !! cache.Repr)
+      && (forall ref | ref in cache.Contents :: this !in cache.Contents[ref].Repr)
+      && this !in cache.Repr
+      && cache.Inv()
+      && (forall ref | ref in cache.Contents :: cache.Contents[ref].Inv())
+    }
+
+    protected function I() : map<BT.G.Reference, IM.Node>
+    reads this, Repr
+    requires Inv()
+    {
+      map ref | ref in cache.Contents :: cache.Contents[ref].I()
+    }
+
+    method GetOpt(ref: BT.G.Reference)
+    returns (node: Option<Node>)
+    requires Inv()
+    ensures node.Some? ==> node.value.Inv()
+    ensures node.Some? ==> ref in I()
+    ensures node.Some? ==> node.value.I() == I()[ref]
+    ensures node.None? ==> ref !in I()
+    {
+      node := cache.Get(ref);
+    }
+
+    lemma LemmaSizeEqCount()
+    ensures |I()| == |cache.Contents|
+
+    method Insert(ref: BT.G.Reference, node: Node)
+    requires Inv()
+    requires node.Inv()
+    requires Repr !! node.Repr
+    requires |I()| <= 0x10000
+    modifies Repr
+    ensures Inv()
+    ensures I() == old(I()[ref := node.I()])
+    ensures forall o | o in Repr :: o in old(Repr) || o in old(node.Repr) || fresh(o)
+    {
+      LemmaSizeEqCount();
+      var _ := cache.Insert(ref, node);
+      assert cache.Contents[ref] == node;
+      Repr := {this} + cache.Repr + MutCacheBucketRepr();
+
+      assert Inv();
+    }
+  }
+
+  // Some helpful lemmas
+
+  /*lemma LemmaReprCacheInsert(cache: map<BT.G.Reference, Node>, ref: BT.G.Reference, node: Node, s: Variables)
+  requires s.cache.Contents == cache[ref := node]
+  requires CacheRepr(cache) !! node.Repr
+  requires CacheRepr(cache) !! s.NonBucketsRepr()
+  requires node.Repr !! s.NonBucketsRepr()
+  requires CacheReprInv_(cache)
+  requires BucketListReprInv(node.buckets)
+  ensures CacheRepr(s.cache.Contents) !! s.NonBucketsRepr()
+  ensures CacheReprInv_(s.cache.Contents)
+  ensures BucketsInv_(s.cache.Contents, CacheRepr(s.cache.Contents))*/
+
+  /*method CacheInsert(k: M.Constants, s: Variables, ref: BT.G.Reference, node: Node)
+  requires s.W()
+  requires s.ready
+  requires node.Repr !! s.Repr()
+  requires WFNode(node)
+  requires |s.cache.Contents| <= MaxCacheSize();
+  modifies s.Repr()
+  ensures s.W()
+  ensures forall o | o in s.Repr() :: fresh(o) || o in old(s.Repr()) || o in old(node.Repr)
+  ensures s.I() == old(s.I()).(cache := old(s.I()).cache[ref := INode(node)])
+  {
+    var _ := s.cache.Insert(ref, node);
+
+    s.uucketRepr := CacheRepr(s.cache.Contents);
+
+    reveal_BucketListReprInv();
+    reveal_CacheRepr();
+    reveal_Cache_();
+    reveal_CacheReprInv_();
+  }*/
+
+}
